tests/lean/run/smt_rsimp.lean
@@ -1,0 +1,19 @@
+constant p {α} : α → α → Prop
+axiom pax {α} : ∀ n : α, p n n
+
+open tactic
+
+meta def check_expr (p : pexpr) (t : expr) : tactic unit :=
+do e ← to_expr p, guard (t = e)
+
+meta def check_target (p : pexpr) : tactic unit :=
+target >>= check_expr p
+
+example (s t : list nat) (h : t = s) : p (s ++ []) ([] ++ t) :=
+begin [smt]
+  add_simp_lemmas,
+  ematch,
+  rsimp,
+  check_target `(p s s),
+  apply pax
+end
